src/Pipit.System.Base.fst
@@ -3,247 +3,274 @@ module Pipit.System.Base
 
 module PM = Pipit.Prop.Metadata
 
-noeq
-type checks (state: Type) = {
-  assumptions: state -> prop;
-  obligations: state -> prop;
+let type_join (t1 t2: option Type): option Type =
+  match t1, t2 with
+  | Some o1, Some o2 -> Some (o1 & o2)
+  | None, o2 -> o2
+  | o1, None -> o1
+
+let option_type_sem (t: option Type): Type =
+  match t with
+  | Some t -> t
+  | None   -> unit
+
+let type_join_fst (#t1 #t2: option Type) (v: option_type_sem (type_join t1 t2)): option_type_sem t1 =
+ match t1, t2 with
+  | Some o1, Some o2 -> fst #(option_type_sem t1) #(option_type_sem t2) v
+  | None, o2 -> ()
+  | o1, None -> v
+
+let type_join_snd (#t1 #t2: option Type) (v: option_type_sem (type_join t1 t2)): option_type_sem t2 =
+ match t1, t2 with
+  | Some o1, Some o2 -> snd #(option_type_sem t1) #(option_type_sem t2) v
+  | None, o2 -> v
+  | o1, None -> ()
+
+let type_join_tup (#t1 #t2: option Type) (v1: option_type_sem t1) (v2: option_type_sem t2): option_type_sem (type_join t1 t2) =
+ match t1, t2 with
+  | Some o1, Some o2 -> (v1, v2)
+  | None, o2 -> v2
+  | o1, None -> v1
+
+let prop_join (o1 o2: option prop): option prop =
+  match o1, o2 with
+  | Some o1, Some o2 -> Some (o1 /\ o2)
+  | None, o2 -> o2
+  | o1, None -> o1
+
+let option_prop_sem (t: option prop): prop =
+  match t with
+  | Some t -> t
+  | None   -> True
+
+
+noeq type checks = {
+  assumptions: option prop;
+  obligations: option prop;
 }
 
+noeq
+type step_result (state: option Type) (result: Type) = {
+  s:    option_type_sem state;
+  v:    result;
+  chck: checks;
+}
 
 (* Step functions are relations so that we can express contracts, which are underspecified.
    The recursive dependency for recursive binders XMu is easier to express as a
    relation too. The result type is `prop`, rather than a computational boolean,
    because composing the relations requires existential quantifiers. *)
 noeq
-type system (input: Type) (state: Type) (result: Type) = {
-  init: state -> prop;
+type system (input: Type) (oracle: option Type) (state: option Type) (result: Type) = {
+  init: option_type_sem state;
 
   step:
     (* Values of input variables *)
     i: input ->
+    o: option_type_sem oracle ->
     (* Starting state *)
-    s: state ->
-    (* New state *)
-    s': state ->
-    (* Return value *)
-    r: result ->
-    prop;
-
-  (* Properties to check *)
-  chck: checks state;
+    s: option_type_sem state ->
+    step_result state result;
 }
 
-let map_checks (#state #state': Type) (f: state' -> state) (chck: checks state): checks state' = {
-  assumptions = (fun s -> chck.assumptions (f s));
-  obligations = (fun s -> chck.obligations (f s));
+let checks_none: checks = {
+  assumptions = None;
+  obligations = None;
 }
 
-let checks_none (state: Type): checks state = {
-  assumptions = (fun s -> True);
-  obligations = (fun s -> True);
+let checks_assumption (f: prop): checks = {
+  assumptions = Some f;
+  obligations = None;
 }
 
-let checks_assumption (#state: Type) (f: state -> prop): checks state = {
-  assumptions = (fun s -> f s);
-  obligations = (fun s -> True);
+let checks_obligation (f: prop): checks = {
+  assumptions = None;
+  obligations = Some f;
 }
 
-let checks_obligation (#state: Type) (f: state -> prop): checks state = {
-  assumptions = (fun s -> True);
-  obligations = (fun s -> f s);
-}
-
-let checks_of_prop (#state: Type) (status: PM.prop_status) (f: state -> prop): checks state =
+let checks_of_prop (status: PM.prop_status) (f: prop): checks =
   match status with
   | PM.PSValid   -> checks_assumption f
   | PM.PSUnknown -> checks_obligation f
 
-let checks_join (#state: Type) (c1 c2: checks state): checks state = {
-  assumptions = (fun s -> c1.assumptions s /\ c2.assumptions s);
-  obligations = (fun s -> c1.obligations s /\ c2.obligations s);
+let checks_join (c1 c2: checks): checks = {
+  assumptions = prop_join c1.assumptions c2.assumptions;
+  obligations = prop_join c1.obligations c2.obligations;
 }
 
-let rec system_steps
-  (#input #state #result: Type)
-  (t: system input state result)
-  (inputs: list (input & state & result))
-  (s': state): prop =
-  match inputs with
-  | [] -> t.init s'
-  | ((i, s, r) :: inputs') ->
-    system_steps t inputs' s /\
-    t.step i s s' r
+// let rec system_steps
+//   (#input #oracle #result: Type)
+//   (#state: option Type)
+//   (t: system input oracle state result)
+//   (inputs: list (input & oracle & option_type_sem state & result))
+//   (s': option_type_sem state): prop =
+//   match inputs with
+//   | [] -> t.init == s'
+//   | ((i, o, s, r) :: inputs') ->
+//     system_steps t inputs' s /\
+//     t.step i s s' r
 
 
-let rec system_stepn
-  (#input #state #result: Type)
-  (t: system input state result)
-  (inputs: list (input & result))
-  (s': state): prop =
-  match inputs with
-  | [] -> t.init s'
-  | ((row, r) :: inputs') ->
-    exists (s0: state).
-    system_stepn t inputs' s0 /\
-    t.step row s0 s' r
+// let rec system_stepn
+//   (#input #state #result: Type)
+//   (t: system input state result)
+//   (inputs: list (input & result))
+//   (s': state): prop =
+//   match inputs with
+//   | [] -> t.init s'
+//   | ((row, r) :: inputs') ->
+//     exists (s0: state).
+//     system_stepn t inputs' s0 /\
+//     t.step row s0 s' r
 
-let system_const (#input #result: Type) (v: result): system input unit result =
-  { init = (fun s -> True);
-    step = (fun i s s' r -> r == v);
-    chck = checks_none unit;
+let system_const (#input #result: Type) (v: result): system input None None result =
+  { init = ();
+    step = (fun i o s -> { s = (); v = v; chck = checks_none; });
   }
 
-let system_check (#input #state: Type)
+let system_check (#input: Type) (#oracle #state: option Type)
   (name: string)
   (status: PM.prop_status)
-  (t1: system input state bool):
-       system input (bool & state) bool =
-  { init = (fun s -> fst s == true /\ t1.init (snd s));
-    step = (fun i s s' r ->
-        t1.step i (snd s) (snd s') r /\
-        // TODO: the property result (fst s') should be anded with (fst s) so it means *always* prop
-        fst s' = r);
-    chck =
-      (checks_of_prop status (fun s -> fst s == true))
-      `checks_join`
-      (map_checks snd t1.chck);
+  (t1: system input oracle state bool):
+       system input oracle state bool =
+  { init = t1.init;
+    step = (fun i o s ->
+      let s1 = t1.step i o s in
+      {
+        s = s1.s;
+        v = s1.v;
+        chck = s1.chck `checks_join` checks_of_prop status (s1.v == true);
+      });
   }
 
-let system_contract_instance (#input #state1 #state2: Type)
+let system_contract_instance (#input: Type)
+  (#oracle1 #oracle2 #state1 #state2: option Type)
   (status: PM.prop_status)
-  (tr: system input state1 bool)
-  (tg: system ('a & input) state2 bool):
-       system input ((bool & bool) & (state1 & state2)) 'a =
-  { init = (fun s -> fst (fst s) == true /\ snd (fst s) == true /\ tr.init (fst (snd s)) /\ tg.init (snd (snd s)));
-    step = (fun i s s' r ->
-        // TODO: the property results (fst (fst s')) and (snd (fst s')) should be anded with their corresponding values in s, so
-        // that the property means *always* prop.
-        // However, this requires some existentials, and I'm not totally convinced it's necessary since (fst (fst s')) is always an obligation
-        tr.step i      (fst (snd s)) (fst (snd s')) (fst (fst s')) /\
-        tg.step (r, i) (snd (snd s)) (snd (snd s')) (snd (fst s')));
-    chck =
-      checks_of_prop status (fun s -> fst (fst s) == true)
-      `checks_join`
-      checks_of_prop PM.PSValid (fun s -> fst (fst s) == true ==> snd (fst s) == true)
-      `checks_join`
-      (map_checks (fun s -> fst (snd s)) tr.chck)
-      `checks_join`
-      (map_checks (fun s -> snd (snd s)) tg.chck);
+  (tr: system input oracle1 state1 bool)
+  (tg: system ('a & input) oracle2 state2 bool):
+       system input (Some 'a `type_join` (oracle1 `type_join` oracle2)) (state1 `type_join` state2) 'a =
+  { init = tr.init `type_join_tup` tg.init;
+    step = (fun i vo s ->
+        let v  = type_join_fst vo in
+        let o  = type_join_snd vo in
+        let o1 = type_join_fst o in
+        let o2 = type_join_snd o in
+        let s1 = type_join_fst s in
+        let s2 = type_join_snd s in
+        let stp1 = tr.step     i  o1 s1 in
+        let stp2 = tg.step (v, i) o2 s2 in
+        let rprop = stp1.v == true in
+        let gprop = stp2.v == true in
+        {
+          s    = type_join_tup stp1.s stp2.s;
+          v    = v;
+          chck = checks_assumption (rprop ==> gprop) `checks_join`
+                 checks_of_prop status rprop `checks_join`
+                 stp1.chck `checks_join` stp2.chck;
+        });
   }
 
-let system_contract_definition (#input #state1 #state2 #state3: Type)
-  (tr: system input state1 bool)
-  (tg: system ('a & input) state2 bool)
-  (ti: system input state3 'a):
-       system input ((bool & bool) & (state1 & (state2 & state3))) 'a =
-  { init = (fun s -> fst (fst s) == true /\ snd (fst s) == true /\ tr.init (fst (snd s)) /\ tg.init (fst (snd (snd s))) /\ ti.init (snd (snd (snd s))));
-    step = (fun i s s' r ->
-        // TODO: the property results (fst (fst s')) and (snd (fst s')) should be anded with their corresponding values in s, so
-        // that the property means *always* prop.
-        // However, this requires some existentials, and I'm not totally convinced it's necessary since (fst (fst s')) is always an obligation
-        tr.step i      (fst (snd s)) (fst (snd s')) (fst (fst s')) /\
-        tg.step (r, i) (fst (snd (snd s))) (fst (snd (snd s'))) (snd (fst s')) /\
-        ti.step i      (snd (snd (snd s))) (snd (snd (snd s'))) r
-        );
-    chck =
-      { assumptions = (fun s -> fst (fst s) == true);
-        obligations = (fun s -> snd (fst s) == true) }
-      `checks_join`
-      (map_checks (fun s -> fst (snd s)) tr.chck)
-      `checks_join`
-      (map_checks (fun s -> fst (snd (snd s))) tg.chck)
-      `checks_join`
-      (map_checks (fun s -> snd (snd (snd s))) ti.chck);
+let system_contract_definition (#input: Type)
+  (#oracle1 #oracle2 #oracle3 #state1 #state2 #state3: option Type)
+  (tr: system input oracle1 state1 bool)
+  (tg: system ('a & input) oracle2 state2 bool)
+  (ti: system input oracle3 state3 'a):
+       system input (oracle1 `type_join` (oracle2 `type_join` oracle3)) (state1 `type_join` (state2 `type_join` state3)) 'a =
+  { init = tr.init `type_join_tup` (tg.init `type_join_tup` ti.init);
+    step = (fun i o s ->
+        let o1 = type_join_fst o in
+        let o2 = type_join_fst (type_join_snd o) in
+        let o3 = type_join_snd (type_join_snd o) in
+        let s1 = type_join_fst s in
+        let s2 = type_join_fst (type_join_snd s) in
+        let s3 = type_join_snd (type_join_snd s) in
+
+        let stp3 = ti.step i o3 s3 in
+        let v    = stp3.v          in
+        let stp1 = tr.step i o1 s1 in
+        let stp2 = tg.step (v, i) o2 s2 in
+        let rprop = stp1.v == true in
+        let gprop = stp2.v == true in
+        {
+          s = stp1.s `type_join_tup` (stp2.s `type_join_tup` stp3.s);
+          v = v;
+          chck = checks_obligation gprop `checks_join`
+                 checks_assumption rprop `checks_join`
+                 stp1.chck `checks_join` stp2.chck `checks_join` stp3.chck;
+        });
   }
 
 let system_project (#input #result: Type) (f: input -> result):
-       system input unit result =
-  { init = (fun _ -> True);
-    step = (fun i s s' r -> r == f i);
-    chck = checks_none unit;
+       system input None None result =
+  { init = ();
+    step = (fun i o s ->
+      {
+        s = ();
+        v = f i;
+        chck = checks_none;
+      });
   }
 
-let system_with_input (#input #input' #state #result: Type) (f: input' -> input)
-    (t: system input state result):
-        system input' state result =
+let system_with_input (#input #input' #result: Type)
+    (#oracle #state: option Type)
+    (f: input' -> input)
+    (t: system input oracle state result):
+        system input' oracle state result =
   { init = t.init;
-    step = (fun i s s' r -> t.step (f i) s s' r);
-    chck = t.chck;
+    step = (fun i o s -> t.step (f i) o s);
   }
 
-let system_pre (#input #state1 #v: Type) (init: v)
-  (t1: system input state1 v):
-       system input (state1 & v) v =
-  { init = (fun s -> t1.init (fst s) /\ snd s == init);
-    step = (fun i s s' r ->
-      t1.step i (fst s) (fst s') (snd s') /\ r == snd s);
-    chck = map_checks fst t1.chck;
+let system_pre (#input #value: Type)
+  (#oracle #state: option Type)
+  (init: value)
+  (t1: system input oracle state value):
+       system input oracle (Some value `type_join` state) value =
+  { init = type_join_tup init t1.init;
+    step = (fun i o sv ->
+      let v  = type_join_fst sv in
+      let s1 = type_join_snd sv in
+      let stp1 = t1.step i o s1 in
+      {
+        s = type_join_tup stp1.v stp1.s;
+        v = v;
+        chck = stp1.chck;
+      });
   }
 
-let system_mu (#input #input' #state1 #v: Type)
-  (extend: input -> v -> input')
-  (t1: system input' state1 v):
-       system input state1 v =
+let system_mu (#input #input' #value: Type)
+  (#oracle #state: option Type)
+  (extend: input -> value -> input')
+  (t1: system input' oracle state value):
+       system input (Some value `type_join` oracle) state value =
   { init = t1.init;
-    step = (fun i s s' r -> t1.step (extend i r) s s' r);
-    chck = t1.chck;
+    step = (fun i vo s ->
+      let v = type_join_fst vo in
+      let o = type_join_snd vo in
+      let stp1 = t1.step (extend i v) o s in
+      {
+        s = stp1.s;
+        v = stp1.v;
+        chck = checks_assumption (v == stp1.v) `checks_join` stp1.chck;
+      });
   }
 
-let system_let (#input #input' #state1 #state2 #v1 #v2: Type)
+let system_let (#input #input' #v1 #v2: Type)
+  (#oracle1 #oracle2 #state1 #state2: option Type)
   (extend: input -> v1 -> input')
-  (t1: system input  state1 v1)
-  (t2: system input' state2 v2):
-       system input (state1 & state2) v2 =
-  { init = (fun s -> t1.init (fst s) /\ t2.init (snd s));
-    step = (fun i s s' r ->
-      let s1 = fst s in
-      let s1' = fst s' in
-      let s2 = snd s in
-      let s2' = snd s' in
-      exists (r1: v1).
-        t1.step i s1 s1' r1 /\
-        t2.step (extend i r1) s2 s2' r);
-    chck = (map_checks fst t1.chck) `checks_join` (map_checks snd t2.chck);
+  (t1: system input oracle1 state1 v1)
+  (t2: system input' oracle2 state2 v2):
+       system input (oracle1 `type_join` oracle2) (state1 `type_join` state2) v2 =
+  { init = type_join_tup t1.init t2.init;
+    step = (fun i o s ->
+      let o1 = type_join_fst o in
+      let o2 = type_join_snd o in
+      let s1 = type_join_fst s in
+      let s2 = type_join_snd s in
+      let stp1 = t1.step i o1 s1 in
+      let stp2 = t2.step (extend i stp1.v) o2 s2 in
+      {
+        s = type_join_tup stp1.s stp2.s;
+        v = stp2.v;
+        chck = stp1.chck `checks_join` stp2.chck;
+      });
   }
-
-(***** Unnecessary combinators? *)
-
-let system_ap2 (#input #state1 #state2 #value1 #value2: Type)
-  (t1: system input state1 (value1 -> value2))
-  (t2: system input state2 value1):
-       system input (state1 & state2) value2 =
-  {
-    init = (fun s -> t1.init (fst s) /\ t2.init (snd s));
-    step = (fun i s s' r ->
-      exists (f: value1 -> value2) (a: value1).
-        t1.step i (fst s) (fst s') f /\
-        t2.step i (snd s) (snd s') a /\
-        r == f a);
-    chck =
-      (map_checks fst t1.chck) `checks_join` (map_checks snd t2.chck);
-  }
-
-let system_map (#input #state1 #value1 #result: Type) (f: value1 -> result)
-  (t1: system input state1 value1):
-       system input state1 result =
-  { init = t1.init;
-    step = (fun i s s' r ->
-      exists (r1: value1).
-       t1.step i s s' r1 /\
-       r == f r1);
-    chck = t1.chck;
-  }
-
-let rec system_map_sem (#input #state1 #value1 #result: Type) (f: value1 -> result)
-  (t1: system input state1 value1)
-  (inputs: list (input & value1))
-  (s': state1):
-    Lemma (requires system_stepn t1 inputs s')
-      (ensures system_stepn (system_map f t1) (List.Tot.map (fun (i,v) -> (i, f v)) inputs) s') =
- match inputs with
- | []  -> ()
- | (i, v) :: is' ->
-   eliminate exists (s0: state1). system_stepn t1 is' s0 /\ t1.step i s0 s' v
-   returns system_stepn (system_map f t1) (List.Tot.map (fun (i,v) -> (i, f v)) inputs) s'
-   with hEx.
-        system_map_sem f t1 is' s0
