src/Pipit.System.Exp.fst
@@ -9,217 +9,72 @@ module CR = Pipit.Context.Row
 module PM = Pipit.Prop.Metadata
 
 open Pipit.System.Base
-open Pipit.System.Det
 
 
-(* A system we get from translating an expression *)
-let xsystem (#t: table) (c: context t) (state: Type) (value: Type) = system (row c) state value
-(* Same, but deterministic *)
-let xdsystem (#t: table) (c: context t) (state: Type) (value: Type) = dsystem (row c) state value
-(* A pure function with no streaming *)
-let xpure (#t: table) (c: context t) (value: Type) = row c -> value
-
-let xsystem_stepn
-  (#tbl: table)
-  (#c: context tbl)
-  (#state #value: Type)
-  (t: xsystem c state value)
-  (streams: list (row c & value))
-  (s': state): prop =
-  system_stepn t streams s'
-
-let rec exp_is_pure (#t: table) (#c: context t) (#a: t.ty) (e: exp t c a): Tot bool (decreases e) =
+let rec state_of_exp (#t: table) (#c: context t) (#a: t.ty) (e: exp t c a): Tot (option Type) (decreases e) =
   match e with
-  | XBase _ -> true
-  | XApps e1 -> exp_apps_is_pure e1
-  | XFby v e1 -> false
-  | XMu e1 -> false
-  | XLet b e1 e2 -> exp_is_pure e1 && exp_is_pure e2
-  // Checks are conceptually wrapped in an "always", so we don't treat them as pure
-  | XCheck name e1 -> false
-  | XContract status rely guar impl ->
-    false
-
-and exp_apps_is_pure (#t: table) (#c: context t) (#a: funty t.ty) (e: exp_apps t c a): Tot bool (decreases e) =
-  match e with
-  | XPrim _ -> true
-  | XApp f e -> exp_apps_is_pure f && exp_is_pure e
-
-
-
-let rec state_of_exp (#t: table) (#c: context t) (#a: t.ty) (e: exp t c a): Tot Type (decreases e) =
-  if exp_is_pure e then unit else
-  match e with
-  | XBase _ -> unit
+  | XBase _ -> None
   | XApps e1 -> state_of_exp_apps e1
-  | XFby v e1 -> state_of_exp e1 & t.ty_sem a
+  | XFby v e1 -> Some (t.ty_sem a) `type_join` state_of_exp e1
   | XMu e1 -> state_of_exp e1
-  | XLet b e1 e2 -> state_of_exp e1 & state_of_exp e2
-  | XCheck name e1 -> bool & state_of_exp e1
+  | XLet b e1 e2 -> state_of_exp e1 `type_join` state_of_exp e2
+  | XCheck name e1 -> state_of_exp e1
   // Contracts do not expose their body in abstract mode, so we only need state of rely and guar
   | XContract status rely guar impl ->
-    (bool & bool) & (state_of_exp rely & state_of_exp guar)
+    state_of_exp rely `type_join` state_of_exp guar
 
-and state_of_exp_apps (#t: table) (#c: context t) (#a: funty t.ty) (e: exp_apps t c a): Tot Type (decreases e) =
+and state_of_exp_apps (#t: table) (#c: context t) (#a: funty t.ty) (e: exp_apps t c a): Tot (option Type) (decreases e) =
   match e with
-  | XPrim _ -> unit
-  | XApp f e -> state_of_exp e & state_of_exp_apps f
+  | XPrim _ -> None
+  | XApp f e -> state_of_exp e `type_join` state_of_exp_apps f
 
 let state_of_contract_definition (#t: table) (#c: context t) (#a: t.ty)
-  (rely: exp t c t.propty) (guar: exp t (a :: c) t.propty) (impl: exp t c a): Type =
-  (bool & bool) & (state_of_exp rely & (state_of_exp guar & state_of_exp impl))
+  (rely: exp t c t.propty) (guar: exp t (a :: c) t.propty) (impl: exp t c a): option Type =
+  (state_of_exp rely `type_join` (state_of_exp guar `type_join` state_of_exp impl))
 
-let rec dstate_of_exp (#t: table) (#c: context t) (#a: t.ty) (e: exp t c a): Tot Type (decreases e) =
-  if exp_is_pure e then unit else
+
+let rec oracle_of_exp (#t: table) (#c: context t) (#a: t.ty) (e: exp t c a): Tot (option Type) (decreases e) =
   match e with
-  | XBase _ -> unit
-  | XApps e1 -> dstate_of_exp_apps e1
-  | XFby v e1 -> dstate_of_exp e1 & t.ty_sem a
-  | XMu e1 -> dstate_of_exp e1
-  | XLet b e1 e2 -> dstate_of_exp e1 & dstate_of_exp e2
-  | XCheck name e1 -> bool & dstate_of_exp e1
+  | XBase _ -> None
+  | XApps e1 -> oracle_of_exp_apps e1
+  | XFby v e1 -> oracle_of_exp e1
+  | XMu e1 -> Some (t.ty_sem a) `type_join` oracle_of_exp e1
+  | XLet b e1 e2 -> oracle_of_exp e1 `type_join` oracle_of_exp e2
+  | XCheck name e1 -> oracle_of_exp e1
+  // Contracts do not expose their body in abstract mode, so we only need state of rely and guar
   | XContract status rely guar impl ->
-    dstate_of_exp impl
+    Some (t.ty_sem a) `type_join` (oracle_of_exp rely `type_join` oracle_of_exp guar)
 
-and dstate_of_exp_apps (#t: table) (#c: context t) (#a: funty t.ty) (e: exp_apps t c a): Tot Type (decreases e) =
+and oracle_of_exp_apps (#t: table) (#c: context t) (#a: funty t.ty) (e: exp_apps t c a): Tot (option Type) (decreases e) =
   match e with
-  | XPrim _ -> unit
-  | XApp f e -> dstate_of_exp e & dstate_of_exp_apps f
+  | XPrim _ -> None
+  | XApp f e -> oracle_of_exp e `type_join` oracle_of_exp_apps f
 
+let oracle_of_contract_definition (#t: table) (#c: context t) (#a: t.ty)
+  (rely: exp t c t.propty) (guar: exp t (a :: c) t.propty) (impl: exp t c a): option Type =
+  (oracle_of_exp rely `type_join` (oracle_of_exp guar `type_join` oracle_of_exp impl))
 
-let rec exp_is_deterministic (#t: table) (#c: context t) (#a: t.ty) (e: exp t c a): Tot bool (decreases e) =
-  match e with
-  | XBase _ -> true
-  | XApps e1 -> exp_apps_is_deterministic e1
-  | XFby v e1 -> exp_is_deterministic e1
-  | XMu e1 -> exp_is_deterministic e1
-  | XLet b e1 e2 -> exp_is_deterministic e1 && exp_is_deterministic e2
-  | XCheck name e1 -> exp_is_deterministic e1
-  // To express contracts, we want a relational rather than functional system
-  | XContract status rely guar impl ->
-    false
+(* A system we get from translating an expression *)
+let xsystem (#t: table) (#c: context t) (#a: t.ty) (e: exp t c a) = system (row c) (oracle_of_exp e) (state_of_exp e) (t.ty_sem a)
 
-and exp_apps_is_deterministic (#t: table) (#c: context t) (#a: funty t.ty) (e: exp_apps t c a): Tot bool (decreases e) =
-  match e with
-  | XPrim _ -> true
-  | XApp f e -> exp_apps_is_deterministic f && exp_is_deterministic e
-
-let lemma_state_dstate_det (#t: table) (#c: context t) (#a: t.ty) (e: exp t c a { exp_is_deterministic e }):
-  Lemma (state_of_exp e == dstate_of_exp e) =
-  admit ()
-
-let pure_of_exp_base
+let system_of_exp_base
   (#t: table) (#c: context t) (#a: t.ty)
-  (e: exp_base t c a { Causal.causal_base e }):
-    Tot (xpure c (t.ty_sem a)) (decreases e) =
+  (e: exp_base t c a):
+    Tot (xsystem (XBase e)) (decreases e) =
     match e with
-    | XVal v -> (fun _ -> v)
-    | XBVar x -> (fun i -> CR.index (context_sem c) i x)
-    | XVar x -> false_elim ()
-
-let rec pure_of_exp
-  (#t: table) (#c: context t) (#a: t.ty)
-  (e: exp t c a { Causal.causal e /\ exp_is_pure e }):
-    Tot (xpure c (t.ty_sem a)) (decreases e) =
-    match e with
-    | XBase e1 -> pure_of_exp_base e1
-    | XApps e1 ->
-      let t = pure_of_exp_apps e1 (fun r _ -> r) in
-      (fun r -> t () r)
-    | XLet b e1 e2 ->
-      let t1 = pure_of_exp e1 in
-      let t2 = pure_of_exp e2 in
-      (fun i -> let v1 = t1 i in t2 (v1, i))
-    | XFby _ _ | XMu _ | XCheck _ _ | XContract _ _ _ _ ->
-      false_elim ()
-
-and pure_of_exp_apps
-  (#t: table) (#c: context t) (#a: funty t.ty) (#res #inp: Type0)
-  (e: exp_apps t c a { Causal.causal_apps e /\ exp_apps_is_pure e })
-  (f: funty_sem t.ty_sem a -> inp -> res):
-    Tot (inp -> row c -> res) (decreases e) =
-    match e with
-    | XPrim p -> (fun i r -> f (t.prim_sem p) i)
-    | XApp e1 e2 ->
-      let arg = XApp?.arg e in
-      let ret = XApp?.ret e in
-      lemma_funty_sem_FTFun t.ty_sem arg ret;
-      let t1: (t.ty_sem arg & inp) -> row c -> res = pure_of_exp_apps e1 (fun r i -> f (r (fst i)) (snd i)) in
-      let t2: xpure c (t.ty_sem arg) = pure_of_exp e2 in
-      (fun i r -> t1 (t2 r, i) r)
-
-
-// let dsystem_of_exp_base
-//   (#t: table) (#c: context t) (#a: t.ty)
-//   (e: exp_base t c a { Causal.causal_base e }):
-//     Tot (xdsystem c unit (t.ty_sem a)) (decreases e) =
-//     match e with
-//     | XVal v -> dsystem_const v
-//     | XBVar x -> dsystem_project (fun i -> CR.index (context_sem c) i x)
-//     | XVar x -> false_elim ()
-
-
-let rec dsystem_of_exp
-  (#t: table) (#c: context t) (#a: t.ty)
-  (e: exp t c a { Causal.causal e }):
-    Tot (xdsystem c (dstate_of_exp e) (t.ty_sem a)) (decreases e) =
-  // PERF:TRANS: See note: translation complexity
-  if exp_is_pure e
-  then dsystem_project (pure_of_exp e)
-  else
-    match e with
-    | XBase e1 -> false_elim ()
-    | XApps e1 ->
-      let t: dsystem (unit & row c) (dstate_of_exp_apps e1) (t.ty_sem a) = dsystem_of_exp_apps e1 (fun r i -> r) in
-      dsystem_with_input (fun s -> ((), s)) t
-    | XFby v e1 ->
-      dsystem_pre v (dsystem_of_exp e1)
-    | XMu e1 ->
-      let t' = dsystem_of_exp e1 in
-      dsystem_mu_causal #(row c) #(t.ty_sem a & row c) (t.val_default a) (fun i v -> (v, i)) t'
-    | XLet b e1 e2 ->
-      dsystem_let (fun i v -> (v, i)) (dsystem_of_exp e1) (dsystem_of_exp e2)
-    | XCheck status e1 ->
-      dsystem_check "XCheck" status (dsystem_of_exp e1)
-    | XContract status rely guar impl ->
-      dsystem_of_exp impl
-
-and dsystem_of_exp_apps
-  (#t: table) (#c: context t) (#a: funty t.ty) (#res #inp: Type0)
-  (e: exp_apps t c a { Causal.causal_apps e })
-  (f: funty_sem t.ty_sem a -> inp -> res):
-    Tot (dsystem (inp & row c) (dstate_of_exp_apps e) res) (decreases e) =
-    match e with
-    | XPrim p -> dsystem_project  (fun i -> f (t.prim_sem p) (fst i))
-    | XApp e1 e2 ->
-      let arg = XApp?.arg e in
-      let ret = XApp?.ret e in
-      lemma_funty_sem_FTFun t.ty_sem arg ret;
-      let t1: dsystem ((t.ty_sem arg & inp) & row c) _ res = dsystem_of_exp_apps e1 (fun r i -> f (r (fst i)) (snd i)) in
-      let t2: xdsystem c _ (t.ty_sem arg) = dsystem_of_exp e2 in
-      let t2': dsystem (inp & row c) _ (t.ty_sem arg) = dsystem_with_input snd t2 in
-      dsystem_let (fun i v -> ((v, fst i), snd i)) t2' t1
-
-
+    | XVal v -> system_const v
+    | XBVar x -> system_project (fun i -> CR.index (context_sem c) i x)
+    // XXX:TODO: treat as oracle
+    | XVar x -> admit () // false_elim ()
 
 let rec system_of_exp
   (#t: table) (#c: context t) (#a: t.ty)
-  (e: exp t c a { Causal.causal e }):
-    Tot (xsystem c (state_of_exp e) (t.ty_sem a)) (decreases e) =
-  // PERF:TRANS: wrong complexity!
-  // Note: translation complexity:
-  // This has the wrong complexity. We descend into the expression to check if it's deterministic, but each sub-call will also descend.
-  // The right way to do this is probably to create a datatype that can represent both xsystem and xdsystem, and have combinators to join them together.
-  if exp_is_deterministic e
-  then (
-    lemma_state_dstate_det e;
-    system_of_dsystem (dsystem_of_exp e))
-  else
+  (e: exp t c a):
+    Tot (xsystem e) (decreases e) =
     match e with
-    | XBase e1 -> false_elim ()
+    | XBase e1 -> system_of_exp_base e1
     | XApps e1 ->
-      assume (not (exp_is_pure e));
-      let t: system (unit & row c) (state_of_exp_apps e1) (t.ty_sem a) = system_of_exp_apps e1 (fun r i -> r) in
+      let t: system (unit & row c) (oracle_of_exp_apps e1) (state_of_exp_apps e1) (t.ty_sem a) = system_of_exp_apps e1 (fun r i -> r) in
       system_with_input (fun s -> ((), s)) t
     | XFby v e1 ->
       system_pre v (system_of_exp e1)
@@ -227,7 +82,6 @@ let rec system_of_exp
       let t' = system_of_exp e1 in
       system_mu #(row c) #(t.ty_sem a & row c) (fun i v -> (v, i)) t'
     | XLet b e1 e2 ->
-      assume (not (exp_is_pure e));
       system_let (fun i v -> (v, i)) (system_of_exp e1) (system_of_exp e2)
     | XCheck status e1 ->
       system_check "XCheck" status (system_of_exp e1)
@@ -238,26 +92,26 @@ let rec system_of_exp
 
 and system_of_exp_apps
   (#t: table) (#c: context t) (#a: funty t.ty) (#res #inp: Type0)
-  (e: exp_apps t c a { Causal.causal_apps e })
+  (e: exp_apps t c a)
   (f: funty_sem t.ty_sem a -> inp -> res):
-    Tot (system (inp & row c) (state_of_exp_apps e) res) (decreases e) =
+    Tot (system (inp & row c) (oracle_of_exp_apps e) (state_of_exp_apps e) res) (decreases e) =
     match e with
     | XPrim p -> system_project (fun i -> f (t.prim_sem p) (fst i))
     | XApp e1 e2 ->
       let arg = XApp?.arg e in
       let ret = XApp?.ret e in
       lemma_funty_sem_FTFun t.ty_sem arg ret;
-      let t1: system ((t.ty_sem arg & inp) & row c) _ res = system_of_exp_apps e1 (fun r i -> f (r (fst i)) (snd i)) in
-      let t2: xsystem c _ (t.ty_sem arg) = system_of_exp e2 in
-      let t2': system (inp & row c) _ (t.ty_sem arg) = system_with_input snd t2 in
+      let t1: system ((t.ty_sem arg & inp) & row c) _ _ res = system_of_exp_apps e1 (fun r i -> f (r (fst i)) (snd i)) in
+      let t2: system (row c) _ _ (t.ty_sem arg) = system_of_exp e2 in
+      let t2': system (inp & row c) _ _ (t.ty_sem arg) = system_with_input snd t2 in
       system_let (fun i v -> ((v, fst i), snd i)) t2' t1
 
 let system_of_contract
   (#t: table) (#c: context t) (#a: t.ty)
-  (r: exp t       c  t.propty { Causal.causal r })
-  (g: exp t (a :: c) t.propty { Causal.causal g })
-  (i: exp t       c         a { Causal.causal i }):
-    xsystem c (state_of_contract_definition r g i) (t.ty_sem a) =
+  (r: exp t       c  t.propty)
+  (g: exp t (a :: c) t.propty)
+  (i: exp t       c         a):
+    system (row c) (oracle_of_contract_definition r g i) (state_of_contract_definition r g i) (t.ty_sem a) =
   let tr = system_of_exp r in
   let tg = system_of_exp g in
   let ti = system_of_exp i in
