example/Fir.CheckN.fst
@@ -16,8 +16,8 @@ let treal = Pipit.Prim.Vanilla.TReal
 
 type fir_contract (mul: R.real) =
   Check.contract table [treal] treal
-    (Check.exp_of_stream1 (fun i -> abs i <=^ r1))
-    (Check.exp_of_stream2 (fun r i -> abs r <=^ pure mul))
+    (Check.exp_of_stream1 (fun i -> (pure (R.of_int (-1))) <=^ i /\ i <=^ r1))
+    (Check.exp_of_stream2 (fun r i -> r <=^ pure mul))
 
 // type fir_contract' (mul: list R.real) =
 //   Check.contract1 table [treal] treal
@@ -32,28 +32,22 @@ let rec sum_abs (coeffs: list R.real) =
   | [] -> R.zero
   | c::cs' -> R.(r_abs c +. sum_abs cs')
 
+#push-options "--split_queries always"
+
+
 #push-options "--print_full_names"
 let rec fir_body (coeffs: list R.real):
   fir_contract (sum_abs coeffs) =
-  let r = (Check.exp_of_stream1 (fun i -> abs i <=^ r1)) in
-  let g = (Check.exp_of_stream2 (fun r i -> abs r <=^ pure (sum_abs coeffs))) in
-
+  let r = (Check.exp_of_stream1 (fun i -> (pure (R.of_int (-1))) <=^ i /\ i <=^ r1)) in
+  let g = (Check.exp_of_stream2 (fun r i -> r <=^ pure (sum_abs coeffs))) in
   match coeffs with
   | [] ->
     let e = Check.exp_of_stream1 (fun _ -> zero) in
-    assume (Check.contract_system_induct_k1' r g e);
-    // assert (Check.contract_system_induct_k1' r g e) by (T.norm_full ());
+    assert (Check.contract_system_induct_k1' r g e) by (T.norm_full ());
     Check.contract_of_exp1 r g e
   | c :: coeffs' ->
-    let gg = (Check.exp_of_stream2 (fun r i -> abs r <=^ pure R.(r_abs c +. sum_abs coeffs'))) in
-    // assert (g = gg);
     let e = Check.exp_of_stream1 (fun input ->
       let fir' = Check.stream_of_contract1 (fir_body coeffs') (fby 0.0R input) in
       (input *^ pure c) +^ fir') in
-    // assume (Pipit.Exp.Causality.causal r);
-    // assume (Pipit.Exp.Causality.causal gg);
-    // assume (Pipit.Exp.Causality.causal e);
-    // assert (Check.contract_system_induct_k1' r gg e) by (T.norm_full (); T.dump "step");
-    assert (Pipit.System.Ind.base_case (Pipit.System.Exp.system_of_contract r gg e)) by (T.pipit_simplify_products (); T.dump "step");
-    assume (Check.contract_system_induct_k1' r g e);
+    assert (Check.contract_system_induct_k1' r g e) by (T.norm_full ());
     Check.contract_of_exp1 r g e
