src/Pipit.System.Exec.fst
@@ -1,0 +1,69 @@
+(* Executable transition systems *)
+module Pipit.System.Exec
+
+open Pipit.System.Base
+
+noeq
+type esystem (input: Type) (state: option Type) (result: Type) = {
+  init: option_type_sem state;
+
+  step:
+    (* Values of input variables *)
+    i: input ->
+    (* Starting state *)
+    s: option_type_sem state ->
+    (* Updated state and result *)
+    (option_type_sem state & result);
+}
+
+let esystem_const (#input #result: Type) (v: result): esystem input None result =
+  { init = ();
+    step = (fun i s -> ((), v));
+  }
+
+let esystem_project (#input #result: Type) (f: input -> result):
+       esystem input None result =
+  { init = ();
+    step = (fun i s -> ((), f i));
+  }
+
+let esystem_with_input (#input #input' #result: Type) (#state: option Type) (f: input' -> input)
+    (t: esystem input state result):
+        esystem input' state result =
+  { init = t.init;
+    step = (fun i s -> t.step (f i) s);
+  }
+
+let esystem_pre (#input #v: Type) (#state1: option Type) (init: v)
+  (t1: esystem input state1 v):
+       esystem input (Some v `type_join` state1) v =
+  { init = type_join_tup init t1.init;
+    step = (fun i s ->
+      let (s1', v') = t1.step i (type_join_snd s) in
+      (type_join_tup v' s1', type_join_fst s));
+  }
+
+let esystem_mu_causal (#input #input' #v: Type)
+  (#state1: option Type)
+  (bottom: v)
+  (extend: input -> v -> input')
+  (t1: esystem input' state1 v):
+       esystem input state1 v =
+  { init = t1.init;
+    step = (fun i s ->
+      let (s',r) = t1.step (extend i bottom) s in
+      t1.step (extend i r) s);
+  }
+
+let esystem_let (#input #input' #v1 #v2: Type)
+  (#state1 #state2: option Type)
+  (extend: input -> v1 -> input')
+  (t1: esystem input  state1 v1)
+  (t2: esystem input' state2 v2):
+       esystem input (state1 `type_join` state2) v2 =
+  { init = type_join_tup t1.init t2.init;
+    step = (fun i s ->
+      let (s1', r1) = t1.step i (type_join_fst s) in
+      let (s2', r2) = t2.step (extend i r1) (type_join_snd s) in
+      (type_join_tup s1' s2', r2));
+  }
